Examples/arm8_strcasecmp_proof.v
@@ -1,0 +1,462 @@
+(* Nathaniel Simmons, Aaron Hill, Long Nguyen, Ariz Siddiqui
+
+   Code for CS 6335 Language-Based Security Class at UT Dallas
+
+   To run this module, first load and compile:
+   * Picinae_syntax
+   * Picinae_theory
+   * Picinae_finterp
+   * Picinae_statics
+   * Picinae_slogic
+   * Picinae_armv8_pcode
+   * strcasecmp_lo_strcasecmp_armv8
+   (in that order) and then compile this module using menu option
+   Compile->Compile buffer.
+ *)
+
+Require Import Utf8.
+Require Import FunctionalExtensionality.
+Require Import Arith.
+Require Import NArith.
+Require Import ZArith.
+Require Import Lia.
+Require Import Picinae_armv8_pcode.
+Require Import arm8_strcasecmp.
+
+Import ARM8Notations.
+Open Scope N.
+
+(* The ARMv8 lifter models non-writable code. *)
+Theorem strcasecmp_nwc: 
+	forall s2 s1, strcasecmp s1 = strcasecmp s2.
+Proof. 
+	reflexivity. 
+Qed.
+
+(* Example #1: Type safety *)
+Theorem strcasecmp_welltyped: 
+	welltyped_prog arm8typctx strcasecmp.
+Proof.
+  Picinae_typecheck.
+Qed.
+
+Theorem strcaselen_preserves_lr:
+	forall_endstates strcasecmp (fun _ s _ s' => s R_LR = s' R_LR).
+Proof.
+  apply noassign_prog_same.
+  prove_noassign.
+Qed.
+
+Theorem strcasecmp_preserves_readable:
+	forall_endstates strcasecmp (fun _ s _ s' => s A_READ = s' A_READ).
+Proof.
+  apply noassign_prog_same.
+  prove_noassign.
+Qed.
+
+Theorem strcasecmp_preserves_writable:
+	forall_endstates strcasecmp (fun _ s _ s' => s A_WRITE = s' A_WRITE).
+Proof.
+	apply noassign_prog_same.
+	prove_noassign.
+Qed.
+
+(* Define to_lower *)
+Definition tolower (c:N) : N :=
+  if andb (65 <=? c mod 2^32) (c mod 2^32 <=? 90) then (c mod 2^32 .| 32) else c.
+
+(* Define binary-level string equality: *)
+Definition strcaseeq (m: addr -> N) (p1 p2: addr) (k: N) :=
+  ∀ i, i < k -> tolower (m Ⓑ[p1+i]) = tolower (m Ⓑ[p2+i]) /\ 0 < m Ⓑ[p1+i].
+
+Section Invariants.
+
+  Variable sp : N          (* initial stack pointer *).
+  Variable mem : addr -> N (* initial memory state *).
+  Variable raddr : N       (* R_X30 return address *).
+  Variable arg1 : N        (* strcasecmp: R_X0 (1st pointer arg)
+                              tolower: R_X0 input character *).
+  Variable arg2 : N        (* strcasecmp: R_X1 (2nd pointer arg)
+                              tolower: R_X19 (callee-save reg) *).
+  Variable x20 x21 : value (* tolower: R_X20, R_X21 (callee-save regs) *).
+
+  Definition mem' fbytes := setmem 64 LittleE 40 mem (sp ⊖ 48) fbytes.
+
+  (* The post-condition says that interpreting EAX as a signed integer yields
+     a number n whose sign equals the comparison of the kth byte in the two input
+     strings, where the two strings are identical before k, and n may only be
+     zero if the kth bytes are both nil. *)
+  Definition postcondition (s:store) :=
+    ∃ n k fb,
+      s V_MEM64 = Ⓜ(mem' fb) /\
+      s R_X0 = Ⓠn /\
+      strcaseeq (mem' fb) arg1 arg2 k /\
+      (n=0 -> (mem' fb) Ⓑ[arg1+k] = 0) /\ (* if the strings are equal, we're at the end of the strings *)
+      (tolower (mem' fb Ⓑ[arg1+k]) ?= tolower(mem' fb Ⓑ[arg2+k])) = (toZ 32%N n ?= Z0)%Z.
+
+  (* The invariant-set for this property makes minimal assumptions at program-start
+     (address 1048576) except naming registers, and puts a loop-invariant at address 1048600. *)
+  Definition invs T (Inv Post: inv_type T) (NoInv:T) (s:store) (a:addr) : T :=
+    match a with
+    (* Entry, x0 and x1 are the char strings *)
+    | 1048576 => Inv 1 (
+        s R_SP = Ⓠsp /\ s V_MEM64 = Ⓜmem /\
+        s R_X0 = Ⓠarg1 /\ s R_X1 = Ⓠarg2
+      )
+
+    (* loop invariant *)
+    | 1048600 => Inv 1 (∃ fb k,
+        strcaseeq (mem' fb) arg1 arg2 k /\
+        s R_SP = Ⓠ(sp ⊖ 48) /\ s V_MEM64 = Ⓜ(mem' fb) /\
+        s R_X19 = Ⓠ(arg2 ⊕ k) /\ s R_X20 = Ⓠ(arg1 ⊕ k)
+      )
+
+    (* Both letters must be either equal or case equal after toLower *)
+    | 1048688 => Inv 1 (∃ fb k,
+        strcaseeq (mem' fb) arg1 arg2 k /\
+        s R_SP = Ⓠ(sp ⊖ 48) /\ s V_MEM64 = Ⓜ(mem' fb) /\
+        s R_X19 = Ⓠ(arg2 ⊕ k) /\ s R_X20 = Ⓠ(arg1 ⊕ k) /\
+        (tolower(mem' fb Ⓑ[arg1 + k]) = tolower(mem' fb Ⓑ[arg2 + k])) /\
+        mem' fb Ⓑ[arg1 + k] ≠ 0
+      )
+
+    (* One character is null or both are different after toLower *)
+    | 1048648 => Inv 1 (∃ fb k,
+        strcaseeq (mem' fb) arg1 arg2 k /\ (*characters before k matched*)
+        s R_SP = Ⓠ(sp ⊖ 48) /\ s V_MEM64 = Ⓜ(mem' fb) /\
+        s R_X19 = Ⓠ(arg2 ⊕ k) /\ s R_X20 = Ⓠ(arg1 ⊕ k) /\
+          (tolower(mem' fb Ⓑ[arg1 + k]) ≠ tolower(mem' fb Ⓑ[arg2 + k]) \/
+           mem' fb Ⓑ[arg1 + k] = 0)
+      )
+
+    (* Postcondition *)
+    | 1048684 => Post 1 (postcondition s)
+
+    (* tolower entry point *)
+    | 2097152 => Inv 0 (s R_X0 = Ⓠarg1 /\ s R_X19 = Ⓠarg2 /\
+         s R_X20 = x20 /\ s R_X21 = x21 /\
+         s R_X30 = Ⓠraddr /\ s R_SP = Ⓠsp /\ s V_MEM64 = Ⓜmem)
+
+    (* tolower return point *)
+    | 2097168 => Post 0 (s R_X0 = Ⓠ(tolower arg1) /\ s R_X19 = Ⓠarg2 /\
+         s R_X20 = x20 /\ s R_X21 = x21 /\
+         s R_X30 = Ⓠraddr /\ s R_SP = Ⓠsp /\ s V_MEM64 = Ⓜmem)
+
+    | _ => NoInv
+    end.
+
+  Definition exits0 := make_exits 0 strcasecmp invs.
+  Definition invs0 := make_invs 0 strcasecmp invs.
+  Definition exits1 := make_exits 1 strcasecmp invs.
+  Definition invs1 := make_invs 1 strcasecmp invs.
+
+End Invariants.
+
+Lemma tolower_mod:
+  forall c, (tolower c) mod 2^32 = tolower (c mod 2^32).
+Proof.
+  intro. unfold tolower. rewrite mp2_mod_mod. destruct (andb _ _).
+    rewrite <- N.land_ones, N.land_lor_distr_l, N.land_ones, mp2_mod_mod. reflexivity.
+    reflexivity.
+Qed.
+
+Lemma tolower_small:
+  forall w e m a, tolower (getmem w e 1 m a) < 2^8.
+Proof.
+  intros. unfold tolower. destruct (andb _ _).
+    apply lor_bound.
+      rewrite <- getmem_mod_r, mp2_mod_mod_min. apply mp2_mod_lt.
+      reflexivity.
+    apply getmem_bound.
+Qed.
+
+Corollary tolower_byte:
+  forall w e m a, (tolower (getmem w e 1 m a)) mod 2^32 =
+                  tolower (getmem w e 1 m a).
+Proof.
+  intros. rewrite tolower_mod, N.mod_small. reflexivity.
+  etransitivity. apply getmem_bound. reflexivity.
+Qed.
+
+Lemma tolower_test:
+  forall c,
+    (if 25 <=? msub 32 c 65
+     then if c mod 2^32 =? 90 then 0 else 1
+     else 0) =
+    (if andb (65 <=? c mod 2^32) (c mod 2^32 <=? 90) then 0 else 1).
+Proof.
+  intro c. destruct (N.eq_dec (c mod 2^32) 90) as [H1|H1].
+    rewrite <- (msub_mod_l 32 32). rewrite H1. reflexivity. reflexivity.
+    rewrite (proj2 (N.eqb_neq _ _) H1). destruct (65 <=? _) eqn:H2.
+      apply N.leb_le in H2. destruct (_ <=? 90) eqn:H3.
+        rewrite (proj2 (N.leb_gt _ _)).
+          reflexivity.
+          change 25 with (msub 32 90 65). apply msub_lt_mono_r.
+            left. rewrite N.min_l. apply H2. apply N.leb_le, H3.
+            apply N.leb_le, N.le_lteq in H3. destruct H3 as [H3|H3].
+              assumption.
+              contradict H1. assumption.
+        apply N.leb_gt in H3. rewrite msub_nowrap by assumption. rewrite (proj2 (N.leb_le _ _)).
+          reflexivity.
+          apply N.le_add_le_sub_l, N.lt_le_incl, H3.
+      rewrite msub_wrap by apply N.leb_gt, H2. rewrite (proj2 (N.leb_le _ _)).
+        reflexivity.
+        apply N.le_add_le_sub_l. transitivity (2^32). discriminate 1. apply N.le_add_r.
+Qed.
+
+Lemma diff_compare:
+  forall m n (H1: m < 2^8) (H2: n < 2^8),
+    (m ?= n) = (toZ 32%N (msub 32%N m n) ?= 0)%Z.
+Proof.
+  intros.
+  assert (H1': m < 2^32). eapply N.lt_le_trans. apply H1. discriminate.
+  assert (H2': n < 2^32). eapply N.lt_le_trans. apply H2. discriminate.
+  destruct (m ?= n) eqn:H3; symmetry.
+    apply N.compare_eq_iff in H3. subst. rewrite msub_diag. reflexivity.
+    apply (proj2 (Z.compare_lt_iff _ _)), Z.lt_nge.
+      intro H. apply toZ_sign in H. revert H. apply N.le_ngt.
+      rewrite msub_mod_pow2, N.min_id. apply le_msub_iff.
+      right. rewrite !N.mod_small by assumption. split.
+        apply (proj1 (N.compare_lt_iff _ _) H3).
+        transitivity (2^8+2^31).
+          apply N.add_le_mono. apply N.lt_le_incl, H2. discriminate.
+          transitivity (2^32). discriminate. apply N.le_add_r.
+    apply (proj1 (N.compare_gt_iff _ _)) in H3. apply (proj2 (Z.compare_gt_iff _ _)).
+      rewrite msub_nowrap by (rewrite !N.mod_small by assumption; apply N.lt_le_incl, H3).
+      rewrite !N.mod_small by assumption.
+      rewrite (proj1 (toZ_nonneg _ _)); rewrite N.mod_small.
+      rewrite N2Z.inj_sub by apply N.lt_le_incl, H3. apply Z.lt_0_sub, N2Z.inj_lt, H3.
+      1-3: eapply N.le_lt_trans; [apply N.le_sub_l|try assumption].
+      eapply N.lt_le_trans. apply H1. discriminate.
+Qed.
+
+Ltac step := time arm8_step.
+
+Theorem tolower_correctness:
+  forall s sp mem t xs' arg1 arg2 a'
+         (ENTRY: startof t xs' = (Addr 2097152, s))
+         (MDL: models arm8typctx s)
+         (SP: s R_SP = Ⓠsp) (MEM: s V_MEM64 = Ⓜmem)
+         (X0: s R_X0 = Ⓠarg1) (X19: s R_X19 = Ⓠarg2)
+         (X30: s R_X30 = Ⓠa'),
+  satisfies_all strcasecmp (invs0  sp mem a' arg1 arg2 (s R_X20) (s R_X21))
+                           (exits0 sp mem a' arg1 arg2 (s R_X20) (s R_X21)) (xs'::t).
+Proof.
+  (* Start the proof the same way as before. *)
+  intros. apply prove_invs.
+
+  (* Prove the base case similarly. *)
+  simpl. rewrite ENTRY. step. repeat split; assumption.
+
+  (* Change assumptions about s into assumptions about s1. *)
+  intros.
+  eapply startof_prefix in ENTRY; try eassumption.
+  eapply preservation_exec_prog in MDL; try (eassumption || apply strcasecmp_welltyped).
+  clear - PRE MDL. rename t1 into t.
+
+  (* Break the proof into cases, one for each invariant-point. *)
+  destruct_inv 64 PRE.
+
+  (* Address 152 (tolower entry point) *)
+  destruct PRE as [X0 [X19 [X20 [X21 [X30 [SP MEM]]]]]].
+  step. step. step.
+
+    (* Address 164 *)
+    step. repeat split; try assumption.
+    rewrite tolower_test in BC. unfold tolower.
+    destruct (andb _ _). reflexivity. discriminate.
+
+    (* Address 168 *)
+    repeat split; try assumption.
+    rewrite tolower_test in BC. unfold tolower.
+    destruct (andb _ _). discriminate. reflexivity.
+Qed.
+
+(* Our partial correctness theorem makes the following assumptions:
+   (ENTRY) Specify the start address and state of the subroutine.
+   (MDL) Assume that on entry the processor is in a valid state.
+   (ESP) Let esp be the value of the ESP register on entry.
+   (MEM) Let mem be the memory state on entry.
+   From these, we prove that all invariants (including the post-condition) hold
+   true for arbitrarily long executions (i.e., arbitrary t). *)
+Theorem strcmp_partial_correctness:
+  forall s sp mem t s' x' arg1 arg2 a'
+         (ENTRY: startof t (x',s') = (Addr 1048576, s))
+         (MDL: models arm8typctx s)
+         (SP: s R_SP = Ⓠsp) (MEM: s V_MEM64 = Ⓜmem) (X30: s R_X30 = Ⓠa')
+         (RX0: s R_X0 = Ⓠarg1) (RX1: s R_X1 = Ⓠarg2),
+  satisfies_all strcasecmp (invs1  sp mem a' arg1 arg2 (s R_X20) (s R_X21))
+                           (exits1 sp mem a' arg1 arg2 (s R_X20) (s R_X21)) ((x',s')::t).
+Proof.
+  (* Start the proof the same way as before. *)
+  intros. apply prove_invs.
+
+  (* Prove the base case similarly. *)
+  simpl. rewrite ENTRY. step. repeat split; assumption.
+
+  (* Change assumptions about s into assumptions about s1. *)
+  intros.
+  eapply startof_prefix in ENTRY; try eassumption.
+  eapply preservation_exec_prog in MDL; try (eassumption || apply strcasecmp_welltyped).
+  set (x20 := s R_X20) in *. set (x21 := s R_X21) in *. clearbody x20 x21.
+  clear - PRE MDL. rename t1 into t. rename s1 into s.
+
+  (* Break the proof into cases, one for each invariant-point. *)
+  destruct_inv 64 PRE.
+
+  (* Address 1048576: Entry point *)
+  destruct PRE as [MEM [SP [X0 X1]]].
+  step. step. step. step. step. step.
+  generalize_frame mem as fb.
+  exists fb, 0. psimpl. split.
+    intros i LT. destruct i; discriminate.
+    repeat split.
+
+  (* Address 1048600: Main loop *)
+  destruct PRE as [fb [k [SEQ [SP [MEM [X19 X20]]]]]].
+  step. step.
+
+    (* Address 1048648: Reached null terminator in arg1 *)
+    exists fb, k. repeat (reflexivity || assumption || split).
+    right. apply N.eqb_eq, BC.
+
+    (* Address 1048608: Character in arg1 is non-null. *)
+    apply N.eqb_neq in BC.
+    step. step.
+
+      (* Address 1048648: Reached null terminator in arg2 *)
+      apply N.eqb_eq in BC0.
+      exists fb, k. repeat (reflexivity || assumption || split).
+      left. rewrite BC0. change (tolower 0) with 0. unfold tolower.
+      destruct (andb _ _).
+        intro H. apply N.lor_eq_0_iff, proj2 in H. discriminate.
+        assumption.
+
+      (* Address 1048616: Current char in both strings are non-null. *)
+      apply N.eqb_neq in BC0.
+      step. step.
+
+        (* Address 1048688: Equal characters found. *)
+        eexists fb, k. repeat (assumption || reflexivity || split).
+        apply N.eqb_eq in BC1. rewrite BC1. reflexivity.
+
+        (* Address 1048624: Unequal characters found. Call tolower(arg1). *)
+        step.
+        set (s1 := update _ _ _).
+        eapply models_after_steps. eassumption. apply strcasecmp_welltyped. intro MDL1.
+        eapply (perform_call 0). reflexivity.
+        intros. eapply tolower_correctness; (eassumption || reflexivity).
+        reflexivity.
+
+        intros.
+        unfold s1 in PRE. psimpl in PRE.
+        assert (MDL': models arm8typctx s').
+          eapply preservation_exec_prog; try eassumption.
+          apply strcasecmp_welltyped.
+        set (t' := t2++t0++_::t) in *. clearbody s1 t'.
+        set (x21' := s R_X21) in PRE. clearbody x21'.
+        clear - SEQ BC BC0 BC1 PRE MDL'.
+        rename MDL' into MDL. rename t' into t. rename a'0 into a. rename s' into s.
+
+        destruct_inv 64 PRE.
+
+        destruct PRE as [X0 [X19 [X20 [X21 [X30 [SP MEM]]]]]].
+        clear X21 x21'.
+        step. step. step. step.
+
+        (* Another call to tolower *)
+        set (s1 := update _ _ _).
+        eapply models_after_steps. eassumption. apply strcasecmp_welltyped. intro MDL1.
+        eapply (perform_call 0). reflexivity.
+        intros. eapply tolower_correctness; (eassumption || reflexivity).
+        reflexivity.
+
+        intros.
+        unfold s1 in PRE. psimpl in PRE.
+        assert (MDL': models arm8typctx s').
+          eapply preservation_exec_prog; try eassumption.
+          apply strcasecmp_welltyped.
+        set (t' := t2++t0++_::t) in *. clearbody s1 t'.
+        rewrite X20 in PRE.
+        clear - SEQ BC BC0 BC1 PRE MDL'.
+        rename MDL' into MDL. rename t' into t. rename a'0 into a. rename s' into s.
+
+        destruct_inv 64 PRE.
+
+        destruct PRE as [X0 [X19 [X20 [X21 [X30 [SP MEM]]]]]].
+        step. step. step.
+
+          (* Address 1048688: Found equal characters. *)
+          exists fb, k.
+          rewrite !tolower_byte in BC2.
+          repeat first [ assumption | split ].
+          apply N.eqb_eq, BC2.
+
+          (* Address 1048648: Found unequal characters. *)
+          exists fb, k.
+          rewrite !tolower_byte in BC2.
+          repeat first [ assumption | split ].
+          left. apply N.eqb_neq, BC2.
+
+        (* Address 1048648: Loop back to loop invariant *)
+        destruct PRE as [fb [k [SEQ [SP [MEM [X19 [X20 NEQ]]]]]]].
+        step. step.
+
+        set (s1 := update _ _ _).
+        eapply models_after_steps. eassumption. apply strcasecmp_welltyped. intro MDL1.
+        eapply (perform_call 0). reflexivity.
+        intros. eapply tolower_correctness; (eassumption || reflexivity).
+        reflexivity.
+
+        intros.
+        unfold s1 in PRE. psimpl in PRE.
+        set (x21' := s R_X21) in PRE. clearbody x21'.
+        assert (MDL': models arm8typctx s').
+          eapply preservation_exec_prog; try eassumption.
+          apply strcasecmp_welltyped.
+        set (t' := t2++t0++_::t) in *. clearbody s1 t'.
+        clear - SEQ NEQ PRE MDL'.
+        rename MDL' into MDL. rename t' into t. rename a'0 into a. rename s' into s.
+
+        destruct_inv 64 PRE.
+
+        destruct PRE as [X0 [X19 [X20 [X21 [X30 [SP MEM]]]]]].
+        clear X21 x21'.
+        step. step. step. step.
+
+        set (s1 := update _ _ _).
+        eapply models_after_steps. eassumption. apply strcasecmp_welltyped. intro MDL1.
+        eapply (perform_call 0). reflexivity.
+        intros. eapply tolower_correctness; (eassumption || reflexivity).
+        reflexivity.
+
+        intros.
+        unfold s1 in PRE. psimpl in PRE.
+        set (x21' := s R_X21) in PRE. clearbody x21'.
+        assert (MDL': models arm8typctx s').
+          eapply preservation_exec_prog; try eassumption.
+          apply strcasecmp_welltyped.
+        set (t' := t2++t0++_::t) in *. clearbody s1 t'.
+        clear - SEQ NEQ PRE MDL'.
+        rename MDL' into MDL. rename t' into t. rename a'0 into a. rename s' into s.
+
+        destruct_inv 64 PRE.
+
+        destruct PRE as [X0 [X19 [X20 [X21 [X30 [SP MEM]]]]]].
+        clear X21 x21'.
+        step. step. step. step. step.
+        eexists _, k, fb. repeat first [ reflexivity | assumption | split ].
+          intro H. apply msub_move_0_r in H. destruct NEQ as [H'|H'].
+            contradict H'. rewrite !tolower_byte in H. assumption.
+            assumption.
+          apply diff_compare; apply tolower_small.
+
+  (* Address 1048688: Equal, non-nil chars (loop back) *)
+  destruct PRE as [fb [k [SEQ [SP [MEM [X19 [X20 [EQ NN]]]]]]]].
+  step. step. step.
+  exists fb, (k+1). split.
+    rewrite N.add_1_r. intros i H. apply N.lt_succ_r, N.le_lteq in H. destruct H.
+      revert i H. apply SEQ.
+      subst i. split. assumption. apply N.neq_0_lt_0, NN.
+    psimpl. repeat split; assumption.
+Qed.
