windows_build.bat
@@ -29,6 +29,8 @@
 @IF ERRORLEVEL 1 GOTO :ErrorExit
 %coqc% Picinae_amd64.v
 @IF ERRORLEVEL 1 GOTO :ErrorExit
+%coqc% Picinae_armv8_pcode.v
+@IF ERRORLEVEL 1 GOTO :ErrorExit
 @ECHO Picinae build succeeded!
 @GOTO Done
 :ErrorExit
